test/general/nested_struct_with_arrays.c
@@ -11,32 +11,23 @@ typedef struct _s2 {
 } s2;
 
 INCLUDE (
-[@@pulse_unfold] 
-let owns_s2 (x:ref s2) (y:Seq.seq UInt8.t) =
-exists* s2_spec s1_spec.
+[@@pulse_unfold] let owns_s2 (x:ref s2) (y:Seq.seq UInt8.t) = 
+exists* s2_spec s1_spec. 
   s2_pred x s2_spec **
-  freeable x **
   s1_pred s2_spec.field_s1 s1_spec **
-  freeable s2_spec.field_s1 ** 
   (s1_spec.bytes |-> y) **
-  freeable_array s1_spec.bytes
+  freeable x ** 
+  freeable s2_spec.field_s1 ** freeable_array s1_spec.bytes 
 
-ghost
-fn intro_owns_s2 (x:ref s2) s2_spec s1_spec fs1 bytes (y:_)
-requires
-    s2_pred x s2_spec **
-    s1_pred fs1 s1_spec **
-    (bytes |-> y) **
+ghost fn intro_owns_s2 (#x:ref s2) (#y:ref s1) (#z:array UInt8.t) (#bytes:Seq.seq UInt8.t) ()
+requires 
+    s2_pred x ({field_s1=y}) **
+    s1_pred y ({bytes=z}) **
+    (z |-> bytes) **
     freeable x **
-    freeable fs1 ** 
-    freeable_array bytes **
-    pure (s2_spec.field_s1 == fs1) **
-    pure (s1_spec.bytes == bytes)
-ensures owns_s2 x y
-{
-  rewrite each fs1 as s2_spec.field_s1;
-  rewrite each bytes as s1_spec.bytes;
-}
+    freeable y **
+    freeable_array z
+ensures owns_s2 x bytes { rewrite each z as ({bytes=z}).bytes }
 )
 
 void test()
@@ -44,47 +35,30 @@ void test()
     ISARRAY(32) uint8_t *bytes = (uint8_t*)malloc(sizeof(uint8_t)*32);
     s1 x1;
     LEMMA(s1_pack x1);
-    LEMMA(s1_explode x1);
     x1.bytes = bytes;
-    LEMMA(s1_recover x1);
-
-    LEMMA(s1_explode x1);
     x1.bytes = bytes;
-    LEMMA(s1_recover x1);
-
     LEMMA(admit());
 }
 
 
-RETURNS(x: ref s2)
+RETURNS(x: _)
 ENSURES(exists* y. owns_s2 x y)
 s2* mk_s2()
 {
     ISARRAY(32) uint8_t *bytes = (uint8_t*)malloc(sizeof(uint8_t)*32);
     s1 *x1 = (s1*)malloc(sizeof(s1));
-    LEMMA(s1_explode (!x1));
     x1->bytes = bytes;
-    LEMMA(s1_recover (!x1));
     s2 *x2 = (s2*)malloc(sizeof(s2));
-    LEMMA(s2_explode (!x2));
     x2->field_s1 = x1;
-    LEMMA(s2_recover (!x2));
-    LEMMA(intro_owns_s2 (!x2) _ _ _ _ _);
+    LEMMA(intro_owns_s2 ());
     return x2;
 }
 
 PRESERVES(exists* y. owns_s2 x2 y)
 uint8_t read_byte0(s2 *x2)
 {
-    LEMMA(s2_explode(!x2));
     s1 *x1 = x2->field_s1;
-    LEMMA(s1_explode(!x1));
     LEMMA(pts_to_len (!(!(!x1)).bytes));
-    // uint8_t res = x1->bytes[0];
-    // uint8_t *v = x1->bytes;
-    LEMMA(admit());
-    // uint8_t res = v[0];
-    // LEMMA(s1_recover(!x1));
-    // LEMMA(s2_recover(!x2));
-    return 0;
+    uint8_t res = x1->bytes[0];
+    return res;
 }
