test/general/swap_struct_test.c
@@ -15,23 +15,19 @@ ENSURES((u32_pair_struct_pred x { first = 0ul; second = 1ul }))
 u32_pair_struct* new_u32_pair_struct ()
 {
   u32_pair_struct* x = ( u32_pair_struct* )malloc(sizeof(u32_pair_struct));
-  LEMMA(u32_pair_struct_explode !x);
   x->first = 0ul;
   x->second = 1ul;
-  LEMMA(u32_pair_struct_recover !x);
   return x;
 }
 
 
 ERASED_ARG(#s : u32_pair_struct_spec)
 REQUIRES(u32_pair_struct_pred x s)
-ENSURES("exists* (s':u32_pair_struct_spec). u32_pair_struct_pred x s' ** pure (s' == ({first = s.second; second = s.first}))")
+ENSURES(u32_pair_struct_pred x ({first = s.second; second = s.first}))
 void swap_fields(u32_pair_struct *x) {
-  LEMMA(u32_pair_struct_explode !x);
   uint32_t f1 = x->first;
   x->first = x->second;
   x->second = f1;
-  LEMMA(u32_pair_struct_recover !x);
 }
 
 REQUIRES("x |-> 'x")
@@ -46,11 +42,9 @@ void swap_refs(uint32_t *x, uint32_t *y) {
 
 ERASED_ARG(#s : u32_pair_struct_spec)
 REQUIRES(u32_pair_struct_pred x s)
-ENSURES("exists* (s':u32_pair_struct_spec). u32_pair_struct_pred x s' ** pure (s' == {first = s.second; second = s.first})")
+ENSURES(u32_pair_struct_pred x ({first = s.second; second = s.first}))
 void swap_fields_alt(u32_pair_struct *x) { 
-  LEMMA(u32_pair_struct_explode !x);
   swap_refs(&x->first, &x->second); 
-  LEMMA(u32_pair_struct_recover !x);
 }
 
 int main() {
