test/general/swap_struct_test_3.c
@@ -2,61 +2,55 @@
 #include <stdlib.h>
 #include "../include/PulseMacros.h"
 
-struct _u32_pair_struct {
+typedef struct _u32_pair_struct {
   uint32_t first;
   uint32_t second;
-};
+} u32_pair;
 
 
-REQUIRES(emp)
-RETURNS(x:ref _u32_pair_struct)
+RETURNS(x:_)
 ENSURES(freeable x)
-ENSURES((_u32_pair_struct_pred x { first = 0ul; second = 1ul }))
-struct _u32_pair_struct* new_u32_pair_struct ()
+ENSURES(u32_pair_pred x ({ first = 0ul; second = 1ul }))
+u32_pair* new_u32_pair ()
 {
-  struct _u32_pair_struct* x = ( struct _u32_pair_struct* )malloc(sizeof(struct _u32_pair_struct));
-  LEMMA(_u32_pair_struct_explode !x);
+  u32_pair* x = (u32_pair* )malloc(sizeof(u32_pair));
   x->first = 0ul;
   x->second = 1ul;
-  LEMMA(_u32_pair_struct_recover !x);
   return x;
 }
 
-ERASED_ARG(#s : _u32_pair_struct_spec)
-REQUIRES(_u32_pair_struct_pred x s)
-ENSURES("exists* (s':_u32_pair_struct_spec). _u32_pair_struct_pred x s' ** pure (s' == ({first = s.second; second = s.first}))")
-void swap_fields(struct _u32_pair_struct *x) {
-  LEMMA(_u32_pair_struct_explode !x);
+ERASED_ARG(#s : _)
+REQUIRES(u32_pair_pred x s)
+ENSURES(u32_pair_pred x ({first = s.second; second = s.first}))
+void swap_fields(u32_pair *x) {
   uint32_t f1 = x->first;
   x->first = x->second;
   x->second = f1;
-  LEMMA(_u32_pair_struct_recover !x);
 }
 
-REQUIRES("x |-> 'x")
-REQUIRES("y |-> 'y")
-ENSURES("x |-> 'y")
-ENSURES("y |-> 'x")
+ERASED_ARG(#vx #vy:erased _)
+REQUIRES(x |-> vx)
+REQUIRES(y |-> vy)
+ENSURES(x |-> vy)
+ENSURES(y |-> vx)
 void swap_refs(uint32_t *x, uint32_t *y) {
   uint32_t tmp = *x;
   *x = *y;
   *y = tmp;
 }
 
-ERASED_ARG(#s : _u32_pair_struct_spec)
-REQUIRES(_u32_pair_struct_pred x s)
-ENSURES("exists* (s':_u32_pair_struct_spec). _u32_pair_struct_pred x s' ** pure (s' == {first = s.second; second = s.first})")
-void swap_fields_alt(struct _u32_pair_struct *x) { 
-  LEMMA(_u32_pair_struct_explode !x);
+ERASED_ARG(#s : erased _)
+REQUIRES(u32_pair_pred x s)
+ENSURES(u32_pair_pred x ({first = s.second; second = s.first}))
+void swap_fields_alt(u32_pair *x) { 
   swap_refs(&x->first, &x->second); 
-  LEMMA(_u32_pair_struct_recover !x);
 }
 
 int main() {
-  struct _u32_pair_struct *x = new_u32_pair_struct();
+  u32_pair *x = new_u32_pair();
   swap_fields(x);
   swap_fields_alt(x);
-  LEMMA(with vx. assert ((x |-> vx) ** _u32_pair_struct_pred vx {first = 0ul; second = 1ul}));
+  LEMMA(with vx. assert ((x |-> vx) ** u32_pair_pred vx {first = 0ul; second = 1ul}));
   free( x);
   return EXIT_SUCCESS;
 }
