test/snapshots/Swap_struct_test_3.fst
@@ -9,107 +9,104 @@ open Pulse.Lib.C
 
 
 noeq
-type _u32_pair_struct = {
+type u32_pair = {
 first: ref UInt32.t;
 second: ref UInt32.t;
 }
 
 [@@erasable]
 noeq
-type _u32_pair_struct_spec = {
+type u32_pair_spec = {
 first : UInt32.t;
 second : UInt32.t
 
 }
 
-let _u32_pair_struct_pred ([@@@mkey]x:ref _u32_pair_struct) (s:_u32_pair_struct_spec) : slprop =
-exists* (y: _u32_pair_struct). (x |-> y) **
+[@@pulse_unfold]
+let u32_pair_pred ([@@@mkey]x:ref u32_pair) (s:u32_pair_spec) : slprop =
+exists* (y: u32_pair). (x |-> y) **
 (y.first |-> s.first) **
 (y.second |-> s.second)
 
-assume val _u32_pair_struct_spec_default : _u32_pair_struct_spec
+assume val u32_pair_spec_default : u32_pair_spec
 
-assume val _u32_pair_struct_default (_u32_pair_struct_var_spec:_u32_pair_struct_spec) : _u32_pair_struct
+assume val u32_pair_default (u32_pair_var_spec:u32_pair_spec) : u32_pair
 
 ghost
-fn _u32_pair_struct_pack (_u32_pair_struct_var:ref _u32_pair_struct) (#_u32_pair_struct_var_spec:_u32_pair_struct_spec)
-requires _u32_pair_struct_var|-> _u32_pair_struct_default _u32_pair_struct_var_spec
-ensures exists* v. _u32_pair_struct_pred _u32_pair_struct_var v ** pure (v == _u32_pair_struct_var_spec)
+fn u32_pair_pack (u32_pair_var:ref u32_pair) (#u32_pair_var_spec:u32_pair_spec)
+requires u32_pair_var|-> u32_pair_default u32_pair_var_spec
+ensures exists* v. u32_pair_pred u32_pair_var v ** pure (v == u32_pair_var_spec)
 { admit() }
 
 ghost
-fn _u32_pair_struct_unpack (_u32_pair_struct_var:ref _u32_pair_struct)
-requires exists* v. _u32_pair_struct_pred _u32_pair_struct_var v 
-ensures exists* u. _u32_pair_struct_var |-> u
+fn u32_pair_unpack (u32_pair_var:ref u32_pair)
+requires exists* v. u32_pair_pred u32_pair_var v 
+ensures exists* u. u32_pair_var |-> u
 { admit() }
 
-fn _u32_pair_struct_alloc ()
-returns x:ref _u32_pair_struct
+fn u32_pair_alloc ()
+returns x:ref u32_pair
 ensures freeable x
-ensures exists* v. _u32_pair_struct_pred x v
+ensures exists* v. u32_pair_pred x v
 { admit () }
 
-fn _u32_pair_struct_free (x:ref _u32_pair_struct)
+fn u32_pair_free (x:ref u32_pair)
 requires freeable x
-requires exists* v. _u32_pair_struct_pred x v
+requires exists* v. u32_pair_pred x v
 { admit() }
 
 
-ghost fn _u32_pair_struct_explode (x:ref _u32_pair_struct) (#s:_u32_pair_struct_spec)
-requires _u32_pair_struct_pred x s
-ensures exists* (v: _u32_pair_struct). (x |-> v) ** (v.first |-> s.first) ** 
+ghost fn u32_pair_explode (x:ref u32_pair) (#s:u32_pair_spec)
+requires u32_pair_pred x s
+ensures exists* (v: u32_pair). (x |-> v) ** (v.first |-> s.first) ** 
 (v.second |-> s.second)
 
-{unfold _u32_pair_struct_pred}
+{unfold u32_pair_pred}
 
 
 ghost
-fn _u32_pair_struct_recover (x:ref _u32_pair_struct) (#a0 : UInt32.t)
+fn u32_pair_recover (x:ref u32_pair) (#a0 : UInt32.t)
 (#a1 : UInt32.t)
 
-requires exists* (y: _u32_pair_struct). (x |-> y) ** 
+requires exists* (y: u32_pair). (x |-> y) ** 
 (y.first |-> a0) **
 (y.second |-> a1)
-ensures exists* w. _u32_pair_struct_pred x w ** pure (w == {first = a0;
+ensures exists* w. u32_pair_pred x w ** pure (w == {first = a0;
 second = a1})
-{fold _u32_pair_struct_pred x ({first = a0;
+{fold u32_pair_pred x ({first = a0;
 second = a1}) }
 
-fn new_u32_pair_struct ()
-requires emp
-returns x:ref _u32_pair_struct
+fn new_u32_pair ()
+returns x:_
 ensures freeable x
-ensures (_u32_pair_struct_pred x { first = 0ul; second = 1ul })
+ensures u32_pair_pred x ({ first = 0ul; second = 1ul })
 {
-let mut x : (ref _u32_pair_struct) = _u32_pair_struct_alloc ();
-_u32_pair_struct_explode !x;
-Mk_u32_pair_struct?.first (! (! x)) := (uint64_to_uint32 0UL);
-Mk_u32_pair_struct?.second (! (! x)) := (uint64_to_uint32 1UL);
-_u32_pair_struct_recover !x;
+let mut x : (ref u32_pair) = u32_pair_alloc ();
+Mku32_pair?.first (! (! x)) := (uint64_to_uint32 0UL);
+Mku32_pair?.second (! (! x)) := (uint64_to_uint32 1UL);
 (! x);
 }
 
 fn swap_fields
-(x : ( ref _u32_pair_struct) )
-(#s : _u32_pair_struct_spec)
-requires _u32_pair_struct_pred x s
-ensures exists* (s':_u32_pair_struct_spec). _u32_pair_struct_pred x s' ** pure (s' == ({first = s.second; second = s.first}))
+(x : ( ref u32_pair) )
+(#s : _)
+requires u32_pair_pred x s
+ensures u32_pair_pred x ({first = s.second; second = s.first})
 {
-let mut x : (ref _u32_pair_struct) = x;
-_u32_pair_struct_explode !x;
+let mut x : (ref u32_pair) = x;
 let mut f1 : UInt32.t = (! (! (! x)).first);
-Mk_u32_pair_struct?.first (! (! x)) := (! (! (! x)).second);
-Mk_u32_pair_struct?.second (! (! x)) := (! f1);
-_u32_pair_struct_recover !x;
+Mku32_pair?.first (! (! x)) := (! (! (! x)).second);
+Mku32_pair?.second (! (! x)) := (! f1);
 }
 
 fn swap_refs
 (x : ( ref UInt32.t) )
 (y : ( ref UInt32.t) )
-requires x |-> 'x
-requires y |-> 'y
-ensures x |-> 'y
-ensures y |-> 'x
+(#vx #vy:erased _)
+requires x |-> vx
+requires y |-> vy
+ensures x |-> vy
+ensures y |-> vx
 {
 let mut x : (ref UInt32.t) = x;
 let mut y : (ref UInt32.t) = y;
@@ -119,24 +116,22 @@ let mut tmp : UInt32.t = (! (! x));
 }
 
 fn swap_fields_alt
-(x : ( ref _u32_pair_struct) )
-(#s : _u32_pair_struct_spec)
-requires _u32_pair_struct_pred x s
-ensures exists* (s':_u32_pair_struct_spec). _u32_pair_struct_pred x s' ** pure (s' == {first = s.second; second = s.first})
+(x : ( ref u32_pair) )
+(#s : erased _)
+requires u32_pair_pred x s
+ensures u32_pair_pred x ({first = s.second; second = s.first})
 {
-let mut x : (ref _u32_pair_struct) = x;
-_u32_pair_struct_explode !x;
+let mut x : (ref u32_pair) = x;
 (swap_refs (! (! x)).first (! (! x)).second);
-_u32_pair_struct_recover !x;
 }
 
 fn main ()
 returns Int32.t
 {
-let mut x : (ref _u32_pair_struct) = (new_u32_pair_struct ());
+let mut x : (ref u32_pair) = (new_u32_pair ());
 (swap_fields (! x));
 (swap_fields_alt (! x));
-with vx. assert ((x |-> vx) ** _u32_pair_struct_pred vx {first = 0ul; second = 1ul});
-(_u32_pair_struct_free (! x));
+with vx. assert ((x |-> vx) ** u32_pair_pred vx {first = 0ul; second = 1ul});
+(u32_pair_free (! x));
 0l;
 }
