include/pulse/Pulse.Lib.C.UInt32.fst
@@ -1,0 +1,16 @@
+module Pulse.Lib.C.UInt32
+
+include FStar.UInt32
+module U32 = FStar.UInt32
+
+let uint32 = U32.t
+let as_int (x: U32.t) : int = U32.v x
+let fits (op : int -> int -> int) (vx vy : int) : prop =
+  U32.fits (op vx vy)
+let min_uint32 = FStar.UInt.min_int U32.n
+let max_uint32 = FStar.UInt.max_int U32.n
+let (+^) = FStar.UInt32.add
+
+instance inhabited_uint32 : Pulse.Lib.C.Inhabited.inhabited uint32 = {
+  witness = U32.zero
+}
