test/snapshots/Issue38_test_3.fst
@@ -20,6 +20,7 @@ left : Int32.t
 
 }
 
+[@@pulse_unfold]
 let foo_pred ([@@@mkey]x:ref foo) (s:foo_spec) : slprop =
 exists* (y: foo). (x |-> y) **
 (y.left |-> s.left)
