test/snapshots/Nested_struct_with_arrays.fst
@@ -1,0 +1,174 @@
+module Nested_struct_with_arrays
+
+#lang-pulse
+#set-options "--ext pulse:no_admit_diag"
+
+open Pulse
+open Pulse.Lib.C
+
+
+
+noeq
+type s1 = {
+bytes: ref (array UInt8.t);
+}
+
+[@@erasable]
+noeq
+type s1_spec = {
+bytes : array UInt8.t
+
+}
+
+let s1_relations (s:s1_spec) : prop = 
+Pulse.Lib.Array.length s.bytes == 32
+
+[@@pulse_unfold]
+let s1_pred ([@@@mkey]x:ref s1) (s:s1_spec) : slprop =
+exists* (y: s1). (x |-> y) **
+(y.bytes |-> s.bytes)
+** pure (s1_relations s)
+
+assume val s1_spec_default : s1_spec
+
+assume val s1_default (s1_var_spec:s1_spec) : s1
+
+ghost
+fn s1_pack (s1_var:ref s1) (#s1_var_spec:s1_spec)
+requires s1_var|-> s1_default s1_var_spec
+ensures exists* v. s1_pred s1_var v ** pure (v == s1_var_spec)
+{ admit() }
+
+ghost
+fn s1_unpack (s1_var:ref s1)
+requires exists* v. s1_pred s1_var v 
+ensures exists* u. s1_var |-> u
+{ admit() }
+
+fn s1_alloc ()
+returns x:ref s1
+ensures freeable x
+ensures exists* v. s1_pred x v
+{ admit () }
+
+fn s1_free (x:ref s1)
+requires freeable x
+requires exists* v. s1_pred x v
+{ admit() }
+
+
+ghost fn s1_explode (x:ref s1) (#s:s1_spec)
+requires s1_pred x s
+ensures exists* (v: s1). (x |-> v) ** (v.bytes |-> s.bytes)
+
+** pure (s1_relations s)
+{unfold s1_pred}
+
+
+ghost
+fn s1_recover (x:ref s1) (#a0 : (array UInt8.t))
+
+requires exists* (y: s1). (x |-> y) ** 
+(y.bytes |-> a0)** pure (s1_relations {
+bytes = a0})
+
+ensures exists* w. s1_pred x w ** pure (w == {bytes = a0})
+{fold s1_pred x ({bytes = a0}) }
+
+noeq
+type s2 = {
+field_s1: ref (ref s1);
+}
+
+[@@erasable]
+noeq
+type s2_spec = {
+field_s1 : ( ref s1) 
+
+}
+
+[@@pulse_unfold]
+let s2_pred ([@@@mkey]x:ref s2) (s:s2_spec) : slprop =
+exists* (y: s2). (x |-> y) **
+(y.field_s1 |-> s.field_s1)
+
+assume val s2_spec_default : s2_spec
+
+assume val s2_default (s2_var_spec:s2_spec) : s2
+
+ghost
+fn s2_pack (s2_var:ref s2) (#s2_var_spec:s2_spec)
+requires s2_var|-> s2_default s2_var_spec
+ensures exists* v. s2_pred s2_var v ** pure (v == s2_var_spec)
+{ admit() }
+
+ghost
+fn s2_unpack (s2_var:ref s2)
+requires exists* v. s2_pred s2_var v 
+ensures exists* u. s2_var |-> u
+{ admit() }
+
+fn s2_alloc ()
+returns x:ref s2
+ensures freeable x
+ensures exists* v. s2_pred x v
+{ admit () }
+
+fn s2_free (x:ref s2)
+requires freeable x
+requires exists* v. s2_pred x v
+{ admit() }
+
+
+ghost fn s2_explode (x:ref s2) (#s:s2_spec)
+requires s2_pred x s
+ensures exists* (v: s2). (x |-> v) ** (v.field_s1 |-> s.field_s1)
+
+{unfold s2_pred}
+
+
+ghost
+fn s2_recover (x:ref s2) (#a0 : (ref s1))
+
+requires exists* (y: s2). (x |-> y) ** 
+(y.field_s1 |-> a0)
+ensures exists* w. s2_pred x w ** pure (w == {field_s1 = a0})
+{fold s2_pred x ({field_s1 = a0}) }
+
+[@@pulse_unfold] let owns_s2 (x:ref s2) (y:Seq.seq UInt8.t) = exists* s2_spec s1_spec. s2_pred x s2_spec ** s1_pred s2_spec.field_s1 s1_spec ** (s1_spec.bytes |-> y) ** freeable x ** freeable s2_spec.field_s1 ** freeable_array s1_spec.bytes ghost fn intro_owns_s2 (#x:ref s2) (#y:ref s1) (#z:array UInt8.t) (#bytes:Seq.seq UInt8.t) () requires s2_pred x ({field_s1=y}) ** s1_pred y ({bytes=z}) ** (z |-> bytes) ** freeable x ** freeable y ** freeable_array z ensures owns_s2 x bytes { rewrite each z as ({bytes=z}).bytes }
+fn test ()
+{
+let mut size_expr0 : SizeT.t = (uint64_to_sizet (int32_to_uint64 32l));
+let mut bytes : (array UInt8.t) = alloc_array #UInt8.t !size_expr0;
+let mut x1 : s1 = s1_default s1_spec_default;
+s1_pack x1;
+(! x1).bytes := (! bytes);
+(! x1).bytes := (! bytes);
+admit();
+}
+
+fn mk_s2 ()
+returns x: _
+ensures exists* y. owns_s2 x y
+{
+let mut size_expr1 : SizeT.t = (uint64_to_sizet (int32_to_uint64 32l));
+let mut bytes : (array UInt8.t) = alloc_array #UInt8.t !size_expr1;
+let mut x1 : (ref s1) = s1_alloc ();
+Mks1?.bytes (! (! x1)) := (! bytes);
+let mut x2 : (ref s2) = s2_alloc ();
+Mks2?.field_s1 (! (! x2)) := (! x1);
+intro_owns_s2 ();
+(! x2);
+}
+
+fn read_byte0
+(x2 : ( ref s2) )
+preserves exists* y. owns_s2 x2 y
+returns UInt8.t
+{
+let mut x2 : (ref s2) = x2;
+let mut x1 : (ref s1) = (! (! (! x2)).field_s1);
+pts_to_len (!(!(!x1)).bytes);
+let mut res : UInt8.t = (op_Array_Access (! (! (! x1)).bytes) (int32_to_sizet 0l));
+(! res);
+}
